theories/Analysis/AnalysisForwardSSA.v
@@ -1,0 +1,342 @@
+Require Import CSet Le ListUpdateAt Coq.Classes.RelationClasses.
+
+Require Import Plus Util AllInRel Map Terminating.
+Require Import Val Var Env IL Annotation Infra.Lattice.
+Require Import DecSolve LengthEq MoreList Status AllInRel OptionR.
+Require Import Keep Subterm Analysis.
+
+Set Implicit Arguments.
+
+
+Definition anni A (s:stmt) : Type :=
+  match s with
+  | stmtIf _ _ _ => option A * option A
+  | _ => A
+  end.
+
+Definition forwardF (sT:stmt) (Dom:stmt->Type) `{BoundedSemiLattice (Dom sT)}
+           (forward:〔params〕 ->
+                    forall s (ST:subTerm s sT) (d:Dom sT),
+                      Dom sT * 〔Dom sT〕)
+           (ZL:list params)
+           (F:list (params * stmt)) (a:Dom sT)
+           (ST:forall n s, get F n s -> subTerm (snd s) sT)
+  : list (Dom sT * 〔Dom sT〕).
+  revert F ST.
+  fix g 1. intros.
+  destruct F as [|Zs F'].
+  - eapply nil.
+  - econstructor 2.
+    + refine (forward ZL (snd Zs) _ a).
+      eapply (ST 0 Zs); eauto using get.
+    + eapply (g F').
+      eauto using get.
+Defined.
+
+Arguments forwardF [sT] [Dom] {H} {H0} forward ZL F a ST.
+
+Fixpoint forwardF_length (sT:stmt) (Dom:stmt->Type) `{BoundedSemiLattice (Dom sT)} forward
+           (ZL:list params)
+           (F:list (params * stmt)) a
+           (ST:forall n s, get F n s -> subTerm (snd s) sT) {struct F}
+  : length (forwardF forward ZL F a ST) = length F.
+Proof.
+  destruct F as [|Zs F']; simpl; eauto.
+Qed.
+
+Smpl Add
+     match goal with
+     | [ |- context [ ❬@forwardF ?sT ?Dom ?H ?BSL ?f ?ZL ?F ?a ?ST❭ ] ] =>
+       rewrite (@forwardF_length sT Dom H BSL f ZL F a ST)
+     | [ H : context [ ❬@forwardF ?sT ?Dom ?H ?BSL ?f ?ZL ?F ?a ?ST❭ ] |- _ ] =>
+       rewrite (@forwardF_length sT Dom H BSL f ZL F a ST) in H
+     end : len.
+
+Lemma forwardF_length_ass (sT:stmt) (Dom:stmt->Type) `{BoundedSemiLattice (Dom sT)}
+      forward ZL F a ST k
+  : length F = k
+    -> length (forwardF forward ZL F a ST) = k.
+Proof.
+  intros. rewrite forwardF_length, <- H1.
+  repeat rewrite Nat.min_idempotent; eauto.
+Qed.
+
+Hint Resolve @forwardF_length_ass : len.
+
+Lemma anni_let A
+      (st : stmt) (x : nat) (e : exp) (s : stmt)
+      (EQ:st = stmtLet x e s) (d:anni A st) : A.
+Proof.
+  rewrite EQ in d. simpl in *. eauto.
+Defined.
+
+Lemma anni_if A
+      (st : stmt) (e : op) (s t : stmt)
+      (EQ:st = stmtIf e s t) (d:anni A st) : option A * option A.
+Proof.
+  rewrite EQ in d. simpl in *. eauto.
+Defined.
+
+Lemma anni_app A (st : stmt) f Y
+      (EQ:st = stmtApp f Y) (d:anni A st) : A.
+Proof.
+  rewrite EQ in d. simpl in *. eauto.
+Defined.
+
+Arguments anni_if {A} {st} {e} {s} {t} EQ d.
+
+Definition option_extr A (o:option A) f (x:A) :=
+  match o with
+  | Some a => f a
+  | _ => x
+  end.
+
+
+Fixpoint forward (sT:stmt) (Dom: stmt -> Type) `{BoundedSemiLattice (Dom sT)}
+           (ftransform :
+              forall sT, list params ->
+                    forall s, subTerm s sT -> Dom sT -> anni (Dom sT) s)
+           (ZL:list (params)) (st:stmt) (ST:subTerm st sT) (d:Dom sT) {struct st}
+  :  Dom sT * list (Dom sT).
+  refine (
+      match st as st' return st = st' -> Dom sT * list (Dom sT) with
+      | stmtLet x e s as st =>
+        fun EQ =>
+          let d:Dom sT := anni_let (Dom sT) EQ (ftransform sT ZL st ST d) in
+        @forward sT Dom _ _ ftransform ZL s (subTerm_EQ_Let EQ ST) d
+      | stmtIf x s t =>
+        fun EQ =>
+          let an := anni_if EQ (ftransform sT ZL st ST d) in
+          let (ans', ALs) :=
+              match fst an with
+              | Some d => @forward sT Dom _ H0 ftransform ZL s
+                                     (subTerm_EQ_If1 EQ ST) d
+              | _ => (d, (fun _ => bottom) ⊝ ZL)
+              end in
+          let (ant', ALt) :=
+              match snd an with
+              | Some d => @forward sT Dom _ H0 ftransform ZL t
+                                  (subTerm_EQ_If2 EQ ST) d
+              | _ => (d, (fun _ => bottom) ⊝ ZL)
+              end in
+          (join ans' ant', zip join ALs ALt)
+      | stmtApp f Y as st =>
+        fun EQ =>
+          let d := anni_app (Dom sT) EQ (ftransform sT ZL st ST d) in
+          (d, list_update_at ((fun _ => bottom) ⊝ ZL) (counted f) d)
+
+    | stmtReturn x as st =>
+      fun EQ => (d, (fun _ => bottom) ⊝ ZL)
+
+    | stmtFun F t as st =>
+      fun EQ =>
+        let ZL' := List.map fst F ++ ZL in
+        let (ant', ALt) :=
+            @forward sT Dom _ _ ftransform ZL' t (subTerm_EQ_Fun1 EQ ST)
+                                  d in
+        let anF' := forwardF (forward sT Dom _ _ ftransform) ZL' F d
+                            (subTerm_EQ_Fun2 EQ ST) in
+        let AL' := fold_left (zip join) (snd ⊝ anF') ALt in
+        (fold_left join (fst ⊝ anF') ant', drop ❬F❭ AL')
+      end eq_refl).
+Defined.
+
+Lemma fold_list_length A B (f:list B -> (list A * bool) -> list B) (a:list (list A * bool)) (b: list B)
+  : (forall n aa, get a n aa -> ❬b❭ <= ❬fst aa❭)
+    -> (forall aa b, ❬b❭ <= ❬fst aa❭ -> ❬f b aa❭ = ❬b❭)
+    -> length (fold_left f a b) = ❬b❭.
+Proof.
+  intros LEN.
+  general induction a; simpl; eauto.
+  erewrite IHa; eauto 10 using get with len.
+  intros. rewrite H; eauto using get.
+Qed.
+
+Lemma forwardF_get  (sT:stmt) (Dom:stmt->Type) `{BoundedSemiLattice (Dom sT)}
+           (forward:〔params〕 ->
+                     forall s (ST:subTerm s sT) (d:Dom sT),
+                       Dom sT * list (Dom sT))
+           (ZL:list params)
+           (F:list (params * stmt)) a
+           (ST:forall n s, get F n s -> subTerm (snd s) sT) aa n
+           (GetBW:get (forwardF forward ZL F a ST) n aa)
+      :
+        { Zs : params * stmt & {GetF : get F n Zs &
+        { ST' : subTerm (snd Zs) sT | aa = forward ZL (snd Zs) ST' a
+        } } }.
+Proof.
+  eapply get_getT in GetBW.
+  general induction F; inv GetBW.
+  - exists a. simpl. do 4 (eexists; eauto 20 using get).
+  - edestruct IHF as [Zs [? [? ]]]; eauto; dcr; subst.
+    exists Zs. do 4 (eexists; eauto 20 using get).
+Qed.
+
+Lemma get_forwardF  (sT:stmt) (Dom:stmt->Type) `{BoundedSemiLattice (Dom sT)}
+           (forward:〔params〕 ->
+                     forall s (ST:subTerm s sT) (d:Dom sT),
+                       Dom sT * list (Dom sT))
+           (ZL:list params)
+           (F:list (params * stmt)) (a:Dom sT)
+           (ST:forall n s, get F n s -> subTerm (snd s) sT) n Zs
+  :get F n Zs
+   -> { ST' | get (forwardF forward ZL F a ST) n (forward ZL (snd Zs) ST' a) }.
+Proof.
+  intros GetF.
+  eapply get_getT in GetF.
+  general induction GetF; try destruct Zs as [Z s]; simpl.
+  - eexists; econstructor.
+  - edestruct IHGetF; eauto using get.
+Qed.
+
+
+Ltac inv_get_step_analysis_forward :=
+  match goal with
+  | [ H: get (@forwardF ?sT ?Dom ?PO ?BSL ?f ?ZL ?F ?a ?ST) ?n ?x |- _ ]
+    => eapply (@forwardF_get sT Dom PO BSL f ZL F a ST x n) in H;
+      destruct H as [? [? [? ]]]
+  end.
+
+Smpl Add inv_get_step_analysis_forward : inv_get.
+
+
+Lemma fold_list_length' A B (f:list B -> (list A) -> list B) (a:list (list A)) (b: list B)
+  : (forall n aa, get a n aa -> ❬b❭ <= ❬aa❭)
+    -> (forall aa b, ❬b❭ <= ❬aa❭ -> ❬f b aa❭ = ❬b❭)
+    -> length (fold_left f a b) = ❬b❭.
+Proof.
+  intros LEN.
+  general induction a; simpl; eauto.
+  erewrite IHa; eauto 10 using get with len.
+  intros. rewrite H; eauto using get.
+Qed.
+
+Lemma forward_length (sT:stmt) (Dom : stmt -> Type) `{BoundedSemiLattice (Dom sT)}
+      (f: forall sT, list params ->
+                forall s, subTerm s sT -> Dom sT -> anni (Dom sT) s)
+  : forall (s : stmt) (ST:subTerm s sT) (ZL:list params),
+    forall d, ❬snd (forward Dom f ZL ST d)❭ = ❬ZL❭.
+Proof.
+  sind s; destruct s; simpl; intros; eauto with len;
+    repeat let_pair_case_eq; subst; simpl in *; eauto.
+  - repeat cases; repeat simpl_pair_eqs; subst; simpl; eauto with len.
+    simpl. rewrite zip_length2; eauto.
+    repeat rewrite IH; eauto.
+  - intros. rewrite list_update_at_length. eauto with len.
+  - intros.
+    rewrite length_drop_minus.
+    rewrite fold_list_length'.
+    + rewrite IH; eauto. rewrite app_length, map_length. omega.
+    + intros. inv_get. repeat rewrite IH; eauto.
+    + intros. rewrite zip_length; eauto.
+      eapply min_l; eauto.
+Qed.
+
+
+Smpl Add
+     match goal with
+     | [ |- context [ ❬snd (@forward ?sT ?Dom ?H ?BSL ?f ?ZL ?s ?ST ?d)❭ ] ] =>
+       rewrite (@forward_length sT Dom H BSL f s ST ZL d)
+     end : len.
+
+Lemma forward_length_ass
+      (sT:stmt) (Dom : stmt -> Type) `{BoundedSemiLattice (Dom sT)}
+      (f: forall sT, list params ->
+                forall s, subTerm s sT -> Dom sT -> anni (Dom sT) s)
+  : forall (s : stmt) (ST:subTerm s sT) (ZL:list params) k,
+    forall d, ❬ZL❭ = k -> ❬snd (forward Dom f ZL ST d)❭ = k.
+Proof.
+  intros. rewrite forward_length; eauto.
+Qed.
+
+Lemma forward_length_le_ass
+      (sT:stmt) (Dom : stmt -> Type) `{BoundedSemiLattice (Dom sT)}
+      (f: forall sT, list params ->
+                forall s, subTerm s sT -> Dom sT -> anni (Dom sT) s)
+  : forall (s : stmt) (ST:subTerm s sT) (ZL:list params) k,
+    forall d, ❬ZL❭ <= k -> ❬snd (forward Dom f ZL ST d)❭ <= k.
+Proof.
+  intros. rewrite forward_length; eauto.
+Qed.
+
+Lemma forward_length_le_ass_right
+      (sT:stmt) (Dom : stmt -> Type) `{BoundedSemiLattice (Dom sT)}
+      (f: forall sT, list params ->
+                forall s, subTerm s sT -> Dom sT -> anni (Dom sT) s)
+  : forall (s : stmt) (ST:subTerm s sT) (ZL:list params) k,
+    forall d, k <= ❬ZL❭ -> k <= ❬snd (forward Dom f ZL ST d)❭.
+Proof.
+  intros. rewrite forward_length; eauto.
+Qed.
+
+
+Hint Resolve @forward_length_ass forward_length_le_ass forward_length_le_ass_right : len.
+
+Ltac fold_po :=
+  repeat match goal with
+         | [ H : context [ @ann_R ?A ?A (@poLe ?A ?I) ] |- _ ] =>
+           change (@ann_R A A (@poLe A I)) with (@poLe (@ann A) _) in H
+         | [ H : context [ PIR2 poLe ?x ?y ] |- _ ] =>
+           change (PIR2 poLe x y) with (poLe x y) in H
+         | [ |- context [ ann_R poLe ?x ?y ] ] =>
+           change (ann_R poLe x y) with (poLe x y)
+  end.
+
+Instance PO_anni A s `{PartialOrder A}
+  : PartialOrder (anni A s).
+Proof.
+  destruct s; simpl; eauto with typeclass_instances.
+Defined.
+
+Lemma forward_monotone (sT:stmt) (Dom : stmt -> Type) `{BoundedSemiLattice (Dom sT)}
+      (f: forall sT, list params ->
+                forall s, subTerm s sT -> Dom sT -> anni (Dom sT) s)
+      (fMon:forall s (ST ST':subTerm s sT) ZL,
+          forall a b, a ⊑ b -> f sT ZL s ST a ⊑ f sT ZL s ST' b)
+  : forall (s : stmt) (ST ST':subTerm s sT) (ZL:list params),
+    forall (d d' : Dom sT), d ⊑ d' ->
+                           forward Dom f ZL ST d ⊑ forward Dom f ZL ST' d'.
+Proof with eauto using poLe_setTopAnn, poLe_getAnni.
+  intros s.
+  sind s; destruct s; intros ST ST' ZL d d' LE_d; simpl forward;
+    simpl forward; repeat let_pair_case_eq; subst; eauto 10 using @ann_R;
+      try now (econstructor; simpl; eauto using @ann_R).
+  - eapply IH; eauto.
+    (* Coq can't find the instantiation *)
+    eapply (fMon (stmtLet x e s)); eauto.
+  - pose proof (fMon (stmtIf e s1 s2) ST ST' ZL _ _ LE_d).
+    inv H1; simpl. split. admit. admit.
+  - econstructor; eauto. simpl.
+    + eapply (fMon (stmtApp l Y)); eauto.
+    + eapply update_at_poLe.
+      eapply (fMon (stmtApp l Y)); eauto.
+  - split; simpl; fold_po.
+    + admit.
+    + eapply PIR2_drop. eapply PIR2_fold_zip_join.
+      * eapply PIR2_get; eauto with len.
+        intros; inv_get.
+        eapply IH; eauto.
+      * eapply IH; eauto.
+Admitted.
+
+Require Import FiniteFixpointIteration.
+
+Instance makeForwardAnalysis (Dom:stmt -> Type)
+         `{forall s, PartialOrder (Dom s) }
+         (BSL:forall s, BoundedSemiLattice (Dom s))
+         (f: forall sT, list params ->
+                   forall s, subTerm s sT -> Dom sT -> anni (Dom sT) s)
+         (fMon:forall sT s (ST ST':subTerm s sT) ZL,
+             forall a b, a ⊑ b -> f sT ZL s ST a ⊑ f sT ZL s ST' b)
+         (Trm: forall s, Terminating (Dom s) poLt)
+
+  : forall s, Iteration (Dom s) :=
+  {
+    step := fun X : Dom s => fst (forward Dom f nil (subTerm_refl _) X);
+    initial_value := bottom
+  }.
+Proof.
+  - eapply bottom_least.
+  - hnf; intros.
+    eapply (forward_monotone Dom f (fMon s)); eauto.
+Defined.
